```
-- δ^(α+β) ≅ δ^α ⋅ δ^β
-- (∀ α, β, γ : Type)(∃ f : δ^(α+β) → δ^α × δ^β)(∃ f' : δ^α × δ^β → δ^(α+β))[f ∘ f' = id & f' ∘ f = id]

f : δ^(α+β) → δ^α × δ^β -- ((α+β) → δ) → (α → δ) × (β → δ)
f g = (λa.g (inl a), λb.g (inr b))

f' : δ^α × δ^β → δ^(α+β) -- (α → δ) × (β → δ) → (α+β) → δ
f' w = λs.case s of 
  inl a → w·l a
  inr b → w·r b

Parte L:
  Seja w : δ^α × δ^β.
  Calc:
    (f ∘ f') w
    = f (f' w)  [(∘).1]
    = ((λa.(f' w) (inl a)), λb.(f' w) (inr b)) [f.1 g:=(f' w)]
    = (λa.case (inl a) of (inl a → w·l a) (inr b → w·r b), λb.case (inr b) of (inl a → w·l a) (inr b → w·r b)) [f'.1; f'.1]
    = (λa.w·l a, λb.w·r b) [(+)-β]
    = (w.l, w.r)  [(→)-η; (→)-η]
    = w [(×)-η]
    = id w [← ( ) id]

Parte R:
  Seja g : δ^(α+β).
  Calc:
    (f' ∘ f) g
    = f' (f g) [(∘).1]
    = λs.case s of (inl a → (f g)·l a) (inr b → (f g)·r b)  [f'.1]
    = λs.case s of (inl a → (λa.g (inl a)) a) (inr b → (λb.g (inr b)) b)  [f.1·l; f.1·r]
    = λs.case s of (inl a → (λa.(g ∘ inl) a) a) (inr b → (λb.(g ∘ inr) b) b)  [← (∘).1; ← (∘).1]
    = λs.case s of (inl a → (g ∘ inl) a) (inr b → (g ∘ inr) b)  [(→)-η; (→)-η]
    = λs.case s of (inl a → g (inl a)) (inr b → g (inr b))  [(∘)-η; (∘)-η]
    = λs.g s  [← (+)-E]
    = g [(→)-η]
    = id g [← ( ) id]
```