```lean
--(+)-assoc
-- (∀ α, β, γ : Type)[(α + β) + γ ≅ α + (β + γ)]
-- (∀ α, β, γ : Type)(∃ f : (α + β) + γ → α + (β + γ))(∃ f' : α + (β + γ) → (α + β) + γ)[f ∘ f' = id & f' ∘ f = id]

f : (α + β) + γ → α + (β + γ)
f l·s = case s of | l·a → s | r·b → r·l·b
f r·c = r·r·c

f' : α + (β + γ) → (α + β) + γ
f' l·a = l·l·a
f' r·s = case s of | l·b → l·r·b | r·c → s

Parte L:
  Seja s : α + (β + γ).
  Separo em casos de s:
  Caso l·a:
    Calc:
      (f ∘ f') (l·a)
      = f (f' (l·a))
      = f (l·l·a) [f'.1]
      = case of l·a | l·a → l·a | r·b → r·l·b [f.1]
      = l·a [(+)-E]
      = id l·a
  Caso r·s':
    Separo em casos de s':
    Caso l·b:
      Calc:
        (f ∘ f') (r·l·b)
        = f (f' (r·l·b))
        = f (case l·b of | l·b → l·r·b | r·c → l·b)
        = f (l·r·b)
        = case r·b of | l·a → r·b | r·b → r·l·b
        = r·l·b
        = id r·l·b
    Caso r·c:
      Similar.
Parte R:
  Similar.
```