```
-- α^𝟚 ≅ α × α
-- (∀ α : Type)(∃ f : α^𝟚 → α × α)(∃ f' : α × α → α^𝟚)[f ∘ f' = id & f' ∘ f = id]

f : α^𝟚 → α × α -- (𝟚 → α) → α × α
f g = (g fst, g snd)

f' : α × α → α^𝟚 -- α × α → (𝟚 → α)
f' w = λn.case n of (fst → w·l) (snd → w·r)

Parte L:
  Seja w : α × α.
  Calc:
    (f ∘ f') w
    = f (f' w)
    = f (λn.case n of (fst → w·l) (snd → w·r))
    = ((λn.case n of (fst → w·l) (snd → w·r)) fst, (λn.case n of (fst → w·l) (snd → w·r)) snd)
    = ((case fst of (fst → w·l) (snd → w·r)), (case snd of (fst → w·l) (snd → w·r)))
    = (w·l, w·r)
    = w
    = id w

Parte R:
  Seja g : 𝟚 → α.
  Calc:
    (f' ∘ f) g
    = f' (f g)
    = f' (g fst, g snd)
    = λn.case n of (fst → (g fst, g snd)·l) (snd → (g fst, g snd)·r)
    = λn.case n of (fst → g fst) (snd → g snd)
    = λn.g n
    = g
    = id g
```