```lean
-- ℘f(X ∪ Y) = (℘f X) ∪ (℘f Y)
Sejam f : α → β e X, Y : Set α.
Parte (⊆):
  -- x ∈ ℘f(X ∪ Y) ⇒ x ∈ (℘f X) ∪ (℘f Y)
  Sejam b : β,  h : b ∈ ℘f (X ∪ Y). -- h = (∃ a ∈ X ∪ Y)[f a = b]
  -- x ∈ (℘f X) ∪ (℘f Y) = (∃ a ∈ X)[f a = b] ∨ (∃ a ∈ Y)[f a = b]
  De h obtemos a ∈ X ∪ Y, h' : f a = b.
  Caso a ∈ X:
    Imediato por h'.
  Caso a ∈ Y:
    Similar.

Parte (⊇):
  -- x ∈ (℘f X) ∪ (℘f Y) ⇒ x ∈ ℘f(X ∪ Y)
  Sejam b : B, h : b ∈ (℘f X) ∪ (℘f Y). -- h = (∃ a ∈ X)[f a = b] ∨ (∃ a ∈ Y)[f a = b]
  -- b ∈ ℘f(X ∪ Y) = (∃ a ∈ X ∪ Y)[f a = b]
  Caso b ∈ (℘f X):
    De h.l obtemos a ∈ X, h' : f a = b.
    Imediato por h'.
  Caso b ∈ (℘f Y):
    Similar.
```

```lean
-- ℘f(X ∩ Y) = (℘f X) ∩ (℘f Y)
Sejam f : α → β e X, Y : Set α.
Parte (⊆):
  Sejam b : β, h : b ∈ ℘f(X ∩ Y). 
  De h obtemos a : α, h' : a ∈ X ∩ Y e h'' : f a = b.
  Parte L:
    -- (∃ a ∈ X)[f a = b]
    Escolho a. [h'.l]
    Imediato por h''.
  Parte R:
    -- (∃ a ∈ Y)[f a = b]
    Similar.

Parte (⊇):
  Sejam b : β, h : b ∈ (℘f X) ∩ (℘f Y).
  De h.l obtemos a : α, hl1 : a ∈ X, hl2 : f a = b.
  De h.r obtemos a' : α, hr1 : a' ∈ Y, hr2 : f a' = b.
  Caso f inj:
    Calc:
      f a = f a' [(=)-trans]
      a = a'     [f inj]
    Logo, a ∈ X e a ∈ Y.
    Escolho a.
    Imediato por hl2.
  C.c.:
    --  (∃ x, y : α)[f x = f y & x ≠ y]
    Vou demonstrar que X e Y singleton's serve de contraexemplo.
    -- (∃! x)[x ∈ X] & (∃! y)[y ∈ Y]
    -- ¬(∃ a : α)[a ∈ X ∩ Y ∧ f a = b] = (∀ a : α)[a ∉ X ∩ Y ∨ f a ≠ b]
    Sejam x, y : α, h : x ∈ X & y ∈ Y.
    Suponha que f x = f y & x ≠ y.
    Logo, X ∩ Y = ∅ pelo X singleton e Y singleton.
    Logo, x ∉ X ∩ Y.
    Imediato.
```

```lean
  -- ℘f(X \ Y) = (℘f X) \ (℘f Y)
  todo
```

```lean
  -- ℘f(X Δ Y) = (℘f X) Δ (℘f Y)
  todo
```