```lean
Seja G um grupo.
(≈)-rfl
-- (∀ a : G)[a ≈ a]
Seja a : G.
Escolho a.
Calc:
  aaa⁻¹
  = a(aa⁻¹)
  = ae
  = a

(≈)-symm
-- (∀ a, b : G)[a ≈ b ⇒ b ≈ a]
Sejam a, b : G.
Seja h : a ≈ b.
De h obtemos g : G, h' : a = gbg⁻¹.
Escolho g⁻¹.
Calc:
  (g⁻¹)a((g⁻¹)⁻¹)
  = (g⁻¹)ag
  = (g⁻¹)((gb)g⁻¹)g
  = (g⁻¹)(gb)(g⁻¹g)
  = (g⁻¹)(gb)e
  = (g⁻¹)(gb)
  = (g⁻¹)gb
  = eb
  = b

(≈)-trans
-- (∀ a, b, c : G)[a ≈ b ∧ b ≈ c ⇒ a ≈ c]
Sejam a, b, c : G.
Seja h : a ≈ b ∧ b ≈ c.
De h.l obtemos g : G, hl : a = gbg⁻¹.
De h.r obtemos g' : G, hr : b = g'cg'⁻¹.
Escolho gg'.
Calc:
  (gg')c(gg')⁻¹
  = (gg')c((g'⁻¹)(g⁻¹)) [inv_op]
  = g(g'c)((g'⁻¹)(g⁻¹))
  = g((g'c)(g'⁻¹))(g⁻¹)
  = gb(g⁻¹)             [← hr].
  = a                   [← hl]
```