```lean
θ. inv ∘ (_²) = (_²) ∘ inv -- (∀ g : G)[(inv ∘ (_²)) g = ((_²) ∘ inv) g]
Seja G grupo.
Seja g : G.
Calc:
  (inv ∘ (_²)) g 
  = inv (_² g)
  = inv (g²)
  = inv (gg)

  ((_²) ∘ inv) g
  = (_²) (inv g)
  = (inv g)²
  = (inv g)(inv g)
  = inv (gg) [θ. inv (ab) = (inv b)(inv a)]
----------------
θ. inv ∘ (_ⁿ) = (_ⁿ) ∘ inv -- (∀ g : G)(∀ n : ℕ)[(inv ∘ (_ⁿ)) g = ((_ⁿ) ∘ inv) g]
Seja G grupo.
Seja g : G.
Seja n : ℕ.
Por indução no n.
Base: 
  (inv ∘ (_⁰)) g
  = inv (_⁰ g)
  = inv (g⁰)
  = inv e
  = e

  ((_⁰) ∘ inv) g
  = (_⁰) (inv g)
  = (inv g)⁰
  = e
Passo indutivo: -- H.I := (∀ k : ℕ)[inv ∘ (_ᵏ) = (_ᵏ) ∘ inv ⇒ inv ∘ (_⁽ᵏ⁺¹⁾) = (_⁽ᵏ⁺¹⁾) ∘ inv]
Calc:
  (inv ∘ (_⁽ᵏ⁺¹⁾)) g
  = inv ((_⁽ᵏ⁺¹⁾) g)        [(∘).1]
  = inv (g⁽ᵏ⁺¹⁾)
  = inv (g(gᵏ))             [_ⁿ.2]
  = (inv gᵏ)(inv g)         [θ. inv (ab) = (inv b)(inv a)]
  = (inv ((_ᵏ) g))(inv g)   [← (→)-β]
  = ((inv ∘ (_ᵏ)) g)(inv g) [← (∘).1]
  = (((_ᵏ) ∘ inv) g)(inv g) [H.I]
  = ((_ᵏ) (inv g))(inv g)   [(∘).1]
  = ((inv g)ᵏ)(inv g)       
  = (inv g)⁽ᵏ⁺¹⁾            [← _ᵏ.2]
  = (_⁽ᵏ⁺¹⁾) (inv g)        [← (→)-β]
  = ((_⁽ᵏ⁺¹⁾) ∘ inv) g      [← (∘).1]
```